testing windows proofs

x86/proofs/mlkem_reduce.ml
@@ -12,7 +12,8 @@ needs "common/mlkem_mldsa.ml";;
 
 (* print_literal_from_elf "x86/mlkem/mlkem_reduce.o";; *)
 
-let mlkem_reduce_mc = define_assert_from_elf "mlkem_reduce_mc" "x86/mlkem/mlkem_reduce.o"
+let mlkem_reduce_mc = 
+  define_assert_from_elf "mlkem_reduce_mc" "x86/mlkem/mlkem_reduce.o"
 [
   0xf3; 0x0f; 0x1e; 0xfa;  (* ENDBR64 *)
   0xb8; 0x01; 0x0d; 0x01; 0x0d;
@@ -304,7 +305,8 @@ let lemma_rem = prove
 let overall_lemma = prove
  (`!x:int16.
         ival(word_add (word_sub (barred_x86 x) (word 3329))
-                      (word_and (word_ishr (word_sub (barred_x86 x) (word 3329)) 15)
+                      (word_and (word_ishr
+                                  (word_sub (barred_x86 x) (word 3329)) 15)
                                 (word 3329))) =
         ival x rem &3329`,
   REWRITE_TAC[MATCH_MP lemma_rem (CONGBOUND_RULE `barred_x86 x`)] THEN
@@ -315,7 +317,8 @@ let overall_lemma2 = SPEC_ALL overall_lemma;;
 let overall_lemma3 = AP_TERM `iword:int -> (16)word` overall_lemma2 ;;
 let overall_lemma4 = REWRITE_RULE[IWORD_IVAL] overall_lemma3;;
 
-let SIMD_SIMPLIFY_TAC_LOCAL unfold_defs = RULE_ASSUM_TAC(CONV_RULE(SIMD_SIMPLIFY_CONV unfold_defs));;
+let SIMD_SIMPLIFY_TAC_LOCAL unfold_defs = 
+  RULE_ASSUM_TAC(CONV_RULE(SIMD_SIMPLIFY_CONV unfold_defs));;
 
 let helper_lemma = prove
  (`!x:int16. ival(iword(ival x rem &3329):int16) = ival x rem &3329`,
@@ -324,23 +327,26 @@ let helper_lemma = prove
 
 let MLKEM_REDUCE_CORRECT = prove(
   `!a x pc.
-      aligned 32 a /\
-      nonoverlapping (word pc, 854) (a, 512)
-      ==> ensures x86
-            (\s. bytes_loaded s (word pc) (BUTLAST mlkem_reduce_tmc) /\
-                 read RIP s = word pc /\
-                 C_ARGUMENTS [a] s /\
-                 !i. i < 256
-                       ==> read(memory :> bytes16(word_add a (word(2 * i)))) s = x i)
-            (\s. read RIP s = word (pc + 854) /\
-                 !i. i < 256
-                       ==> ival(read(memory :> bytes16(word_add a (word(2 * i)))) s) =
-                           ival(x i) rem &3329)
-            // Registers (and memory locations) that may change after execution
-            (MAYCHANGE [events] ,,
-             MAYCHANGE [memory :> bytes(a,512)] ,,
-             MAYCHANGE [RIP] ,, MAYCHANGE [RAX] ,,
-             MAYCHANGE [ZMM0; ZMM1; ZMM2; ZMM3; ZMM4; ZMM5; ZMM6; ZMM7; ZMM8; ZMM9; ZMM12])`,
+        aligned 32 a /\
+        nonoverlapping (word pc, 854) (a, 512)
+        ==> ensures x86
+             (\s. bytes_loaded s (word pc) (BUTLAST mlkem_reduce_tmc) /\
+                  read RIP s = word pc /\
+                  C_ARGUMENTS [a] s /\
+                  !i. i < 256
+                      ==> read(memory :> bytes16(word_add a (word(2 * i)))) s =
+                          x i)
+             (\s. read RIP s = word (pc + 854) /\
+                  !i. i < 256
+                      ==> ival(read(memory :> bytes16
+                                 (word_add a (word(2 * i)))) s) =
+                          ival(x i) rem &3329)
+             // Registers (and memory locations) that may change after execution
+             (MAYCHANGE [events] ,,
+              MAYCHANGE [memory :> bytes(a,512)] ,,
+              MAYCHANGE [RIP] ,, MAYCHANGE [RAX] ,,
+              MAYCHANGE [ZMM0; ZMM1; ZMM2; ZMM3; ZMM4; ZMM5;
+                         ZMM6; ZMM7; ZMM8; ZMM9; ZMM12])`,
 
   REWRITE_TAC[fst mlkem_reduce_TMC_EXEC] THEN
   REPEAT STRIP_TAC THEN
@@ -364,7 +370,8 @@ let MLKEM_REDUCE_CORRECT = prove(
   STRIP_TAC THEN
 
 
-  (let lemma = WORD_BLAST `(word_zx:int256->int128) x = word_subword x (0,128)` in
+  (let lemma = WORD_BLAST 
+  `(word_zx:int256->int128) x = word_subword x (0,128)` in
   MAP_EVERY (fun n -> X86_STEPS_TAC mlkem_reduce_TMC_EXEC [n] THEN
                       RULE_ASSUM_TAC(REWRITE_RULE[lemma]) THEN
                       SIMD_SIMPLIFY_TAC_LOCAL[barred_x86])
@@ -388,25 +395,28 @@ let MLKEM_REDUCE_CORRECT = prove(
   REWRITE_TAC[helper_lemma]
 );;
 
-let MLKEM_REDUCE_SUBROUTINE_CORRECT = prove
+let MLKEM_REDUCE_NOIBT_SUBROUTINE_CORRECT = prove
  (`!a x pc stackpointer returnaddress.
-      aligned 32 a /\
-      nonoverlapping (word pc, LENGTH mlkem_reduce_tmc) (a, 512) /\
-      nonoverlapping (stackpointer, 8) (a, 512)
-      ==> ensures x86
-            (\s. bytes_loaded s (word pc) mlkem_reduce_tmc /\
-                 read RIP s = word pc /\
-                 read RSP s = stackpointer /\
-                 read (memory :> bytes64 stackpointer) s = returnaddress /\
-                 C_ARGUMENTS [a] s /\
-                 !i. i < 256
-                       ==> read(memory :> bytes16(word_add a (word(2 * i)))) s = x i)
-            (\s. read RIP s = returnaddress /\
-                 read RSP s = word_add stackpointer (word 8) /\
-                 !i. i < 256
-                       ==> ival(read(memory :> bytes16(word_add a (word(2 * i)))) s)= ival(x i) rem &3329)
-             (MAYCHANGE [RSP] ,, MAYCHANGE_REGS_AND_FLAGS_PERMITTED_BY_ABI ,,
-              MAYCHANGE [memory :> bytes(a, 512)])`,
+        aligned 32 a /\
+        nonoverlapping (word pc, LENGTH mlkem_reduce_tmc) (a, 512) /\
+        nonoverlapping (stackpointer, 8) (a, 512)
+        ==> ensures x86
+             (\s. bytes_loaded s (word pc) mlkem_reduce_tmc /\
+                  read RIP s = word pc /\
+                  read RSP s = stackpointer /\
+                  read (memory :> bytes64 stackpointer) s = returnaddress /\
+                  C_ARGUMENTS [a] s /\
+                  !i. i < 256
+                      ==> read(memory :> bytes16(word_add a (word(2 * i)))) s =
+                          x i)
+             (\s. read RIP s = returnaddress /\
+                  read RSP s = word_add stackpointer (word 8) /\
+                  !i. i < 256
+                      ==> ival(read(memory :> bytes16
+                                 (word_add a (word(2 * i)))) s) =
+                          ival(x i) rem &3329)
+              (MAYCHANGE [RSP] ,, MAYCHANGE_REGS_AND_FLAGS_PERMITTED_BY_ABI ,,
+               MAYCHANGE [memory :> bytes(a, 512)])`,
   X86_PROMOTE_RETURN_NOSTACK_TAC mlkem_reduce_tmc MLKEM_REDUCE_CORRECT);;
 
 let MLKEM_REDUCE_SUBROUTINE_CORRECT = prove
@@ -421,11 +431,113 @@ let MLKEM_REDUCE_SUBROUTINE_CORRECT = prove
                   read (memory :> bytes64 stackpointer) s = returnaddress /\
                   C_ARGUMENTS [a] s /\
                   !i. i < 256
-                      ==> read(memory :> bytes16(word_add a (word(2 * i)))) s = x i)
+                      ==> read(memory :> bytes16(word_add a (word(2 * i)))) s =
+                          x i)
+
              (\s. read RIP s = returnaddress /\
                   read RSP s = word_add stackpointer (word 8) /\
                   !i. i < 256
-                      ==> ival(read(memory :> bytes16(word_add a (word(2 * i)))) s)= ival(x i) rem &3329)
+                      ==> ival(read(memory :> bytes16
+                                 (word_add a (word(2 * i)))) s) =
+                          ival(x i) rem &3329)
              (MAYCHANGE [RSP] ,, MAYCHANGE_REGS_AND_FLAGS_PERMITTED_BY_ABI ,,
               MAYCHANGE [memory :> bytes(a, 512)])`,
-  MATCH_ACCEPT_TAC(ADD_IBT_RULE MLKEM_REDUCE_SUBROUTINE_CORRECT));;
+  MATCH_ACCEPT_TAC(ADD_IBT_RULE MLKEM_REDUCE_NOIBT_SUBROUTINE_CORRECT));;
+
+(* ------------------------------------------------------------------------- *)
+(* Correctness of Windows ABI version.                                       *)
+(* ------------------------------------------------------------------------- *)
+print_literal_from_elf "x86/mlkem/mlkem_reduce.obj";; 
+
+let mlkem_reduce_windows_mc = define_from_elf
+    "mlkem_reduce_windows_mc" "x86/mlkem/mlkem_reduce.obj";;
+ 
+let mlkem_reduce_windows_tmc = define_trimmed
+    "mlkem_reduce_windows_tmc" mlkem_reduce_windows_mc;;
+
+let mlkem_reduce_windows_tmc_EXEC = X86_MK_EXEC_RULE mlkem_reduce_windows_tmc;;
+ 
+let MLKEM_REDUCE_WINDOWS_SUBROUTINE_CORRECT = prove
+ (`!a x pc stackpointer returnaddress.
+        aligned 32 a /\
+        nonoverlapping (word pc, LENGTH mlkem_reduce_windows_tmc) (a, 512) /\
+        nonoverlapping (word_sub stackpointer (word 96), 104) (a, 512) /\
+        nonoverlapping (word pc, LENGTH mlkem_reduce_windows_tmc)
+                       (word_sub stackpointer (word 96), 96)
+        ==> ensures x86
+             (\s. bytes_loaded s (word pc) mlkem_reduce_windows_tmc /\
+                  read RIP s = word pc /\
+                  read RSP s = stackpointer /\
+                  read (memory :> bytes64 stackpointer) s = returnaddress /\
+                  WINDOWS_C_ARGUMENTS [a] s /\
+                  !i. i < 256
+                      ==> read(memory :> bytes16(word_add a (word(2 * i)))) s =
+                          x i)
+             (\s. read RIP s = returnaddress /\
+                  read RSP s = word_add stackpointer (word 8) /\
+                  !i. i < 256
+                      ==> ival(read(memory :> bytes16
+                                 (word_add a (word(2 * i)))) s) =
+                          ival(x i) rem &3329)
+              (MAYCHANGE [RSP] ,,
+               WINDOWS_MAYCHANGE_REGS_AND_FLAGS_PERMITTED_BY_ABI ,,
+               MAYCHANGE [memory :> bytes(word_sub stackpointer (word 96), 96)] ,,
+               MAYCHANGE [memory :> bytes(a, 512)])`,
+  REPLICATE_TAC 3 GEN_TAC THEN
+  WORD_FORALL_OFFSET_TAC 96 THEN
+  REPEAT GEN_TAC THEN
+
+  REWRITE_TAC[fst mlkem_reduce_windows_tmc_EXEC] THEN
+  REPEAT STRIP_TAC THEN REWRITE_TAC[WINDOWS_C_ARGUMENTS] THEN
+  REWRITE_TAC[WINDOWS_MAYCHANGE_REGS_AND_FLAGS_PERMITTED_BY_ABI] THEN
+
+  ENSURES_PRESERVED_TAC "rdi_init" `RDI` THEN
+  ENSURES_PRESERVED_TAC "init_xmm6" `ZMM6 :> bottomhalf :> bottomhalf` THEN
+  ENSURES_PRESERVED_TAC "init_xmm7" `ZMM7 :> bottomhalf :> bottomhalf` THEN
+  ENSURES_PRESERVED_TAC "init_xmm8" `ZMM8 :> bottomhalf :> bottomhalf` THEN
+  ENSURES_PRESERVED_TAC "init_xmm9" `ZMM9 :> bottomhalf :> bottomhalf` THEN
+  ENSURES_PRESERVED_TAC "init_xmm12" `ZMM12 :> bottomhalf :> bottomhalf` THEN
+
+  REWRITE_TAC[READ_ZMM_BOTTOM_QUARTER'] THEN
+  REWRITE_TAC(map GSYM
+    [YMM6;YMM7;YMM8;YMM9;YMM12]) THEN
+
+  GHOST_INTRO_TAC `init_ymm6:int256` `read YMM6` THEN
+  GHOST_INTRO_TAC `init_ymm7:int256` `read YMM7` THEN
+  GHOST_INTRO_TAC `init_ymm8:int256` `read YMM8` THEN
+  GHOST_INTRO_TAC `init_ymm9:int256` `read YMM9` THEN
+  GHOST_INTRO_TAC `init_ymm12:int256` `read YMM12` THEN
+
+  GLOBALIZE_PRECONDITION_TAC THEN
+  REPEAT(FIRST_X_ASSUM(SUBST1_TAC o SYM)) THEN
+
+  ENSURES_INIT_TAC "s0" THEN
+  X86_STEPS_TAC mlkem_reduce_windows_tmc_EXEC (1--8) THEN
+
+  MP_TAC(SPECL [`a:int64`; `x:num->int16`; `pc + 39`]
+    MLKEM_REDUCE_CORRECT) THEN
+  ASM_REWRITE_TAC[C_ARGUMENTS; SOME_FLAGS] THEN
+  ANTS_TAC THENL [NONOVERLAPPING_TAC; ALL_TAC] THEN
+
+  X86_BIGSTEP_TAC mlkem_reduce_windows_tmc_EXEC "s9" THENL
+   [FIRST_ASSUM(MATCH_ACCEPT_TAC o MATCH_MP
+     (BYTES_LOADED_SUBPROGRAM_RULE mlkem_reduce_windows_tmc
+     (REWRITE_RULE[BUTLAST_CLAUSES]
+      (AP_TERM `BUTLAST:byte list->byte list` mlkem_reduce_windows_tmc))
+     39));
+    RULE_ASSUM_TAC(CONV_RULE(TRY_CONV RIP_PLUS_CONV))] THEN
+
+  MAP_EVERY ABBREV_TAC
+   [`ymm6_epilog = read YMM6 s9`;
+    `ymm7_epilog = read YMM7 s9`;
+    `ymm8_epilog = read YMM8 s9`;
+    `ymm9_epilog = read YMM9 s9`;
+    `ymm12_epilog = read YMM12 s9`] THEN
+
+  X86_STEPS_TAC mlkem_reduce_windows_tmc_EXEC (10--17) THEN
+
+  RULE_ASSUM_TAC(REWRITE_RULE[MAYCHANGE_ZMM_QUARTER]) THEN
+  RULE_ASSUM_TAC(REWRITE_RULE[MAYCHANGE_YMM_SSE_QUARTER]) THEN
+
+  ENSURES_FINAL_STATE_TAC THEN ASM_REWRITE_TAC[] THEN
+  REPEAT CONJ_TAC THEN CONV_TAC WORD_BLAST);;
